ROOT
@@ -22,6 +22,16 @@ session "TA_Impl_Calc_Prereq" = "TA_Impl" +
   theories [document = false]
     "$AFP/Gabow_SCC/Gabow_SCC_Code"
 
+session "TA_Impl_Refine_Calc_Prereq" = "TA_Impl" +
+  theories [document = false]
+    "$AFP/Gabow_SCC/Gabow_SCC_Code"
+    UPPAAL_State_Networks_Impl
+
 session "TA_All" = "TA_Impl" +
   theories [document = false]
     UPPAAL_State_Networks_Impl_Refine
+
+session "TA_Code" = "TA_Impl_Refine_Calc_Prereq" +
+  theories [document = false]
+    UPPAAL_Reachability_Benchmarks
+
